CollapsingTowers/TwoLevelRec/LogicalEquiv/Fundamental.lean
@@ -3,7 +3,7 @@ import CollapsingTowers.TwoLevelRec.LogicalEquiv.Compatibility
 -- Γ ⊢ e : τ
 -- ————————————————
 -- Γ ⊧ e ≤𝑙𝑜𝑔 e : τ
-theorem typing.fundamental :
+theorem log_rel_typing.fundamental :
   ∀ Γ e τ,
     typing Γ 𝟚 e τ ∅ →
     log_rel_typing Γ e e τ :=
@@ -65,3 +65,48 @@ theorem typing.fundamental :
   case pure => simp
   case reify => simp
   apply Hτ
+
+lemma log_rel_value.fundamental :
+  ∀ k v τ,
+    value v →
+    typing [] 𝟚 v τ ∅ →
+    log_rel_value k v v τ :=
+  by
+  intros k v τ Hvalue Hτ
+  cases k
+  case zero =>
+    have ⟨Hwbt, _⟩ := typing.wbt_pure_at_dyn _ _ _ _ Hτ
+    cases Hvalue
+    case lam e _ =>
+      cases τ
+      case arrow τ𝕒 τ𝕓 φ =>
+        cases φ <;> simp at Hwbt
+        simp only [log_rel_value]
+        constructor; apply Hτ
+        constructor; apply Hτ
+        simp
+      all_goals contradiction
+    case lit n =>
+      cases τ <;> try contradiction
+      simp
+    case code => nomatch Hτ
+  case succ k =>
+    have ⟨_, _, Hsem_expr⟩ := log_rel_typing.fundamental _ _ _ Hτ
+    simp only [log_rel_expr] at Hsem_expr
+    have ⟨r, Hstep, Hsem_value⟩ := Hsem_expr (k + 1) _ _ (log_rel_env.nil _) 0 (by omega) _ Hvalue (stepn_indexed.refl _)
+    rw [← stepn.value_impl_termination _ _ Hvalue Hstep] at Hsem_value
+    apply Hsem_value
+
+lemma log_rel_env.fundamental :
+  ∀ k γ Γ,
+    typing.subst γ Γ →
+    log_rel_env k γ γ Γ :=
+  by
+  intros k γ Γ HτΓ
+  induction HτΓ
+  case nil => apply log_rel_env.nil
+  case cons v γ τ Γ Hvalue Hτ _ IH =>
+    apply log_rel_env.cons
+    . apply log_rel_value.fundamental
+      apply Hvalue; apply Hτ
+    . apply IH
